src/opt/ReorderStep.v
@@ -60,7 +60,6 @@ Proof.
       i. des.
       left. eexists. econs 4; s; eauto.
       * econs. econs. apply surjective_pairing.
-      * reflexivity.
     + hexploit progress_fence_step; eauto. i. des.
       left. eexists. econs 5; s; eauto.
       econs. econs.
@@ -75,6 +74,7 @@ Proof.
     + apply progress_silent_step. auto.
 Grab Existential Variables.
   { auto. }
+  { apply Capability.elt. }
   { apply Capability.elt. }
 Qed.
 
@@ -130,7 +130,7 @@ Qed.
 
 Lemma reorder_read_fulfill
       loc1 ts1 val1 released1 ord1
-      loc2 from2 to2 val2 released2 ord2
+      loc2 from2 to2 val2 releasedc2 releasedm2 ord2
       lc0 mem0
       lc1
       lc2
@@ -138,9 +138,9 @@ Lemma reorder_read_fulfill
       (ORD: Ordering.le Ordering.seqcst ord2 -> Ordering.le Ordering.seqcst ord1 -> False)
       (WF0: Local.wf lc0 mem0)
       (STEP1: Local.read_step lc0 mem0 loc1 ts1 val1 released1 ord1 lc1)
-      (STEP2: Local.fulfill_step lc1 mem0 loc2 from2 to2 val2 released2 ord2 lc2):
+      (STEP2: Local.fulfill_step lc1 mem0 loc2 from2 to2 val2 releasedc2 releasedm2 ord2 lc2):
   exists lc1',
-    <<STEP1: Local.fulfill_step lc0 mem0 loc2 from2 to2 val2 released2 ord2 lc1'>> /\
+    <<STEP1: Local.fulfill_step lc0 mem0 loc2 from2 to2 val2 releasedc2 releasedm2 ord2 lc1'>> /\
     <<STEP2: Local.read_step lc1' mem0 loc1 ts1 val1 released1 ord1 lc2>>.
 Proof.
   inv STEP1. inv STEP2. ss.
@@ -156,7 +156,7 @@ Admitted.
 
 Lemma reorder_read_write
       loc1 ts1 val1 released1 ord1
-      loc2 from2 to2 val2 released2 ord2
+      loc2 from2 to2 val2 releasedc2 releasedm2 ord2
       lc0 mem0
       lc1 mem1
       lc2
@@ -164,9 +164,9 @@ Lemma reorder_read_write
       (ORD: Ordering.le Ordering.seqcst ord2 -> Ordering.le Ordering.seqcst ord1 -> False)
       (WF0: Local.wf lc0 mem0)
       (STEP1: Local.read_step lc0 mem0 loc1 ts1 val1 released1 ord1 lc1)
-      (STEP2: Local.write_step lc1 mem0 loc2 from2 to2 val2 released2 ord2 lc2 mem1):
+      (STEP2: Local.write_step lc1 mem0 loc2 from2 to2 val2 releasedc2 releasedm2 ord2 lc2 mem1):
   exists lc1',
-    <<STEP1: Local.write_step lc0 mem0 loc2 from2 to2 val2 released2 ord2 lc1' mem1>> /\
+    <<STEP1: Local.write_step lc0 mem0 loc2 from2 to2 val2 releasedc2 releasedm2 ord2 lc1' mem1>> /\
     <<STEP2: Local.read_step lc1' mem1 loc1 ts1 val1 released1 ord1 lc2>>.
 Proof.
   inv STEP2.
@@ -213,7 +213,7 @@ Proof.
 Admitted.
 
 Lemma reorder_fulfill_read
-      loc1 from1 to1 val1 released1 ord1
+      loc1 from1 to1 val1 releasedc1 releasedm1 ord1
       loc2 ts2 val2 released2 ord2
       lc0 mem0
       lc1
@@ -222,11 +222,11 @@ Lemma reorder_fulfill_read
       (ORD1: Ordering.le ord1 Ordering.relaxed)
       (ORD2: Ordering.le ord2 Ordering.relaxed)
       (WF0: Local.wf lc0 mem0)
-      (STEP1: Local.fulfill_step lc0 mem0 loc1 from1 to1 val1 released1 ord1 lc1)
+      (STEP1: Local.fulfill_step lc0 mem0 loc1 from1 to1 val1 releasedc1 releasedm1 ord1 lc1)
       (STEP2: Local.read_step lc1 mem0 loc2 ts2 val2 released2 ord2 lc2):
   exists lc1',
     <<STEP1: Local.read_step lc0 mem0 loc2 ts2 val2 released2 ord2 lc1'>> /\
-    <<STEP2: Local.fulfill_step lc1' mem0 loc1 from1 to1 val1 released1 ord1 lc2>>.
+    <<STEP2: Local.fulfill_step lc1' mem0 loc1 from1 to1 val1 releasedc1 releasedm1 ord1 lc2>>.
 Proof.
   inv STEP1. inv STEP2. ss.
   exploit ReorderCommit.write_read; try apply COMMIT; try apply COMMIT0; eauto.
@@ -240,17 +240,17 @@ Proof.
 Admitted.
 
 Lemma reorder_fulfill_promise
-      loc1 from1 to1 val1 released1 ord1
+      loc1 from1 to1 val1 releasedc1 releasedm1 ord1
       loc2 from2 to2 val2 released2
       lc0 mem0
       lc1
       lc2 mem2
       (WF0: Local.wf lc0 mem0)
-      (STEP1: Local.fulfill_step lc0 mem0 loc1 from1 to1 val1 released1 ord1 lc1)
+      (STEP1: Local.fulfill_step lc0 mem0 loc1 from1 to1 val1 releasedc1 releasedm1 ord1 lc1)
       (STEP2: Local.promise_step lc1 mem0 loc2 from2 to2 val2 released2 lc2 mem2):
   exists lc1',
     <<STEP1: Local.promise_step lc0 mem0 loc2 from2 to2 val2 released2 lc1' mem2>> /\
-    <<STEP2: Local.fulfill_step lc1' mem2 loc1 from1 to1 val1 released1 ord1 lc2>>.
+    <<STEP2: Local.fulfill_step lc1' mem2 loc1 from1 to1 val1 releasedc1 releasedm1 ord1 lc2>>.
 Proof.
   inv STEP1. inv STEP2. ss.
   exploit ReorderMemory.fulfill_promise; try apply MEMORY; try apply WF0; eauto. i. des.
@@ -263,19 +263,19 @@ Proof.
 Qed.
 
 Lemma reorder_fulfill_fulfill
-      loc1 from1 to1 val1 released1 ord1
-      loc2 from2 to2 val2 released2 ord2
+      loc1 from1 to1 val1 releasedc1 releasedm1 ord1
+      loc2 from2 to2 val2 releasedc2 releasedm2 ord2
       lc0 mem0
       lc1
       lc2
       (LOC: loc1 <> loc2)
       (ORD1: Ordering.le ord1 Ordering.relaxed)
       (WF0: Local.wf lc0 mem0)
-      (STEP1: Local.fulfill_step lc0 mem0 loc1 from1 to1 val1 released1 ord1 lc1)
-      (STEP2: Local.fulfill_step lc1 mem0 loc2 from2 to2 val2 released2 ord2 lc2):
+      (STEP1: Local.fulfill_step lc0 mem0 loc1 from1 to1 val1 releasedc1 releasedm1 ord1 lc1)
+      (STEP2: Local.fulfill_step lc1 mem0 loc2 from2 to2 val2 releasedc2 releasedm2 ord2 lc2):
   exists lc1',
-    <<STEP1: Local.fulfill_step lc0 mem0 loc2 from2 to2 val2 released2 ord2 lc1'>> /\
-    <<STEP2: Local.fulfill_step lc1' mem0 loc1 from1 to1 val1 released1 ord1 lc2>>.
+    <<STEP1: Local.fulfill_step lc0 mem0 loc2 from2 to2 val2 releasedc2 releasedm2 ord2 lc1'>> /\
+    <<STEP2: Local.fulfill_step lc1' mem0 loc1 from1 to1 val1 releasedc1 releasedm1 ord1 lc2>>.
 Proof.
   inv STEP1. inv STEP2. ss.
   exploit ReorderMemory.fulfill_fulfill; try apply FULFILL; try apply FULFILL0. i. des.
@@ -290,19 +290,19 @@ Proof.
 Admitted.
 
 Lemma reorder_fulfill_write
-      loc1 from1 to1 val1 released1 ord1
-      loc2 from2 to2 val2 released2 ord2
+      loc1 from1 to1 val1 releasedc1 releasedm1 ord1
+      loc2 from2 to2 val2 releasedc2 releasedm2 ord2
       lc0 mem0
       lc1
       lc2 mem2
       (LOC: loc1 <> loc2)
       (ORD1: Ordering.le ord1 Ordering.relaxed)
       (WF0: Local.wf lc0 mem0)
-      (STEP1: Local.fulfill_step lc0 mem0 loc1 from1 to1 val1 released1 ord1 lc1)
-      (STEP2: Local.write_step lc1 mem0 loc2 from2 to2 val2 released2 ord2 lc2 mem2):
+      (STEP1: Local.fulfill_step lc0 mem0 loc1 from1 to1 val1 releasedc1 releasedm1 ord1 lc1)
+      (STEP2: Local.write_step lc1 mem0 loc2 from2 to2 val2 releasedc2 releasedm2 ord2 lc2 mem2):
   exists lc1',
-    <<STEP1: Local.write_step lc0 mem0 loc2 from2 to2 val2 released2 ord2 lc1' mem2>> /\
-    <<STEP2: Local.fulfill_step lc1' mem2 loc1 from1 to1 val1 released1 ord1 lc2>>.
+    <<STEP1: Local.write_step lc0 mem0 loc2 from2 to2 val2 releasedc2 releasedm2 ord2 lc1' mem2>> /\
+    <<STEP2: Local.fulfill_step lc1' mem2 loc1 from1 to1 val1 releasedc1 releasedm1 ord1 lc2>>.
 Proof.
   inv STEP2.
   - exploit reorder_fulfill_fulfill; eauto. i. des.
@@ -344,7 +344,7 @@ Qed.
 
 Lemma reorder_fence_fulfill
       ordr1 ordw1
-      loc2 from2 to2 val2 released2 ord2
+      loc2 from2 to2 val2 releasedc2 releasedm2 ord2
       lc0 mem0
       lc1
       lc2
@@ -352,9 +352,9 @@ Lemma reorder_fence_fulfill
       (ORDW1: Ordering.le ordw1 Ordering.relaxed)
       (WF0: Local.wf lc0 mem0)
       (STEP1: Local.fence_step lc0 mem0 ordr1 ordw1 lc1)
-      (STEP2: Local.fulfill_step lc1 mem0 loc2 from2 to2 val2 released2 ord2 lc2):
+      (STEP2: Local.fulfill_step lc1 mem0 loc2 from2 to2 val2 releasedc2 releasedm2 ord2 lc2):
   exists lc1',
-    <<STEP1: Local.fulfill_step lc0 mem0 loc2 from2 to2 val2 released2 ord2 lc1'>> /\
+    <<STEP1: Local.fulfill_step lc0 mem0 loc2 from2 to2 val2 releasedc2 releasedm2 ord2 lc1'>> /\
     <<STEP2: Local.fence_step lc1' mem0 ordr1 ordw1 lc2>>.
 Proof.
   inv STEP1. inv STEP2. ss.
@@ -373,7 +373,7 @@ Admitted.
 
 Lemma reorder_fence_write
       ordr1 ordw1
-      loc2 from2 to2 val2 released2 ord2
+      loc2 from2 to2 val2 releasedc2 releasedm2 ord2
       lc0 mem0
       lc1
       lc2 mem2
@@ -381,9 +381,9 @@ Lemma reorder_fence_write
       (ORDW1: Ordering.le ordw1 Ordering.relaxed)
       (WF0: Local.wf lc0 mem0)
       (STEP1: Local.fence_step lc0 mem0 ordr1 ordw1 lc1)
-      (STEP2: Local.write_step lc1 mem0 loc2 from2 to2 val2 released2 ord2 lc2 mem2):
+      (STEP2: Local.write_step lc1 mem0 loc2 from2 to2 val2 releasedc2 releasedm2 ord2 lc2 mem2):
   exists lc1',
-    <<STEP1: Local.write_step lc0 mem0 loc2 from2 to2 val2 released2 ord2 lc1' mem2>> /\
+    <<STEP1: Local.write_step lc0 mem0 loc2 from2 to2 val2 releasedc2 releasedm2 ord2 lc1' mem2>> /\
     <<STEP2: Local.fence_step lc1' mem2 ordr1 ordw1 lc2>>.
 Proof.
   inv STEP2.
